Games/gameLib/Zermelo_Symm.lean
@@ -12,3 +12,361 @@ Note to self:
 
 Try easier Zermelo with a symmetric win-loose game
 -/
+
+inductive Symm_Game_World.has_WL (g : Symm_Game_World α β) : Prop where
+| wf : g.is_fst_win → g.has_WL
+| ws : g.is_snd_win → g.has_WL
+
+
+def Symm_Game_World.world_after_fst {α β : Type u} (g : Symm_Game_World α β)
+  (fst_act : β) : Symm_Game_World α β := -- act not required to be legal
+  {g with init_game_state := g.transition [] fst_act }
+  -- maybe swap fst and snd notions ? Cause we expect snd player to go fst now
+
+
+
+@[simp]
+lemma Symm_Game_World.world_after_fst_init {α β : Type u} (g : Symm_Game_World α β)
+  (fst_act : β) : (g.world_after_fst fst_act).init_game_state = g.transition [] fst_act :=
+  by rfl
+
+@[simp]
+lemma Symm_Game_World.world_after_fst_law {α β : Type u} (g : Symm_Game_World α β)
+  (fst_act : β) : (g.world_after_fst fst_act).law = g.law :=
+  by rfl
+
+@[simp]
+lemma Symm_Game_World.world_after_fst_win_states {α β : Type u} (g : Symm_Game_World α β)
+  (fst_act : β) : (g.world_after_fst fst_act).win_states = g.win_states :=
+  by rfl
+
+
+@[simp]
+lemma Symm_Game_World.world_after_fst_snd_win_states {α β : Type u} (g : Symm_Game_World α β)
+  (fst_act : β) : (g.world_after_fst fst_act).win_states = g.win_states :=
+  by rfl
+
+
+
+instance (l : List α): Decidable (l = []) :=
+  by
+  match l with
+  | [] => apply isTrue ; rfl
+  | x :: L => apply isFalse ; exact List.cons_ne_nil x L
+
+
+lemma Symm_Game_World.History_of_preconditioned'
+  (g: Symm_Game_World α β)
+  (fst_act: β)
+  (f_strat s_strat : Strategy α β)
+  (turn : ℕ):
+  let fst_strat : Strategy α β := (fun ini hist => if hist = [] then fst_act else s_strat (g.world_after_fst fst_act).init_game_state (hist.dropLast)) ;
+  let snd_strat : Strategy α β := (fun ini hist => f_strat (g.world_after_fst fst_act).init_game_state (hist.dropLast)) ;
+  History_on_turn g.init_game_state fst_strat snd_strat (turn + 1) =
+  (History_on_turn (g.world_after_fst fst_act).init_game_state f_strat s_strat turn) ++ [fst_act] :=
+  by
+  intro fst_strat snd_strat
+  induction' turn with t ih
+  · dsimp [History_on_turn, Turn_fst]
+    rw [if_pos (by decide), if_pos (by rfl)]
+  · dsimp only [History_on_turn] at *
+    by_cases q : Turn_fst (t+1)
+    · rw [Turn_fst_not_step] at q
+      rw [if_neg q] at *
+      rw [← Turn_fst_not_step] at q
+      rw [if_pos q, if_pos q] at *
+      rw [List.cons_append, ← ih]
+      congr
+      dsimp at ih
+      rw [← Symm_Game_World.world_after_fst_init] at ih
+      rw [ih]
+      rw [List.dropLast_concat]
+    · rw [if_neg q, if_neg q] at *
+      rw [Turn_fst_not_step, not_not] at q
+      rw [if_pos q] at *
+      rw [if_neg (by apply List.cons_ne_nil)]
+      rw [List.cons_append, ← ih]
+      congr
+      dsimp at ih
+      rw [← Symm_Game_World.world_after_fst_init] at ih
+      rw [ih]
+      rw [List.dropLast_concat]
+
+-- TDOD: rephrase ↓ with ↑
+
+def Symm_Game_World.law_blind_fst' (g : Symm_Game_World α β) : Prop :=
+  ∀ f_strat s_strat: Strategy α β, ∀ fst_act : β, g.law [] fst_act →
+  let fst_strat : Strategy α β := (fun ini hist => if hist = [] then fst_act else s_strat (g.world_after_fst fst_act).init_game_state (hist.dropLast)) ;
+  let snd_strat : Strategy α β := (fun ini hist => f_strat (g.world_after_fst fst_act).init_game_state (hist.dropLast)) ;
+  ∀ turn : ℕ, ∀ act : β, g.law (History_on_turn (g.world_after_fst fst_act).init_game_state f_strat s_strat turn) act
+    ↔ g.law (History_on_turn g.init_game_state fst_strat snd_strat (turn + 1)) act
+
+def Symm_Game_World.law_blind_snd' (g : Symm_Game_World α β) : Prop :=
+  ∀ f_strat s_strat: Strategy α β, ∀ fst_act : β, g.law [] fst_act →
+  let fst_strat : Strategy α β := (fun ini hist => if hist = [] then fst_act else s_strat (g.world_after_fst fst_act).init_game_state (hist.dropLast)) ;
+  let snd_strat : Strategy α β := (fun ini hist => f_strat (g.world_after_fst fst_act).init_game_state (hist.dropLast)) ;
+  ∀ turn : ℕ, ∀ act : β, g.law (History_on_turn (g.world_after_fst fst_act).init_game_state f_strat s_strat turn) act
+    ↔ g.law (History_on_turn g.init_game_state fst_strat snd_strat (turn + 1)) act
+
+
+def Symm_Game_World.law_blind' (g : Symm_Game_World α β) : Prop :=
+ g.law_blind_fst' ∧ g.law_blind_snd'
+
+
+def Symm_Game_World.transition_blind_fst (g : Symm_Game_World α β) : Prop :=
+  ∀ f_strat s_strat: Strategy α β, ∀ fst_act : β, g.law [] fst_act →
+  let fst_strat : Strategy α β := (fun ini hist => if hist = [] then fst_act else s_strat (g.world_after_fst fst_act).init_game_state (hist.dropLast)) ;
+  let snd_strat : Strategy α β := (fun ini hist => f_strat (g.world_after_fst fst_act).init_game_state (hist.dropLast)) ;
+  ∀ turn : ℕ, ∀ act : β, g.transition (History_on_turn (g.world_after_fst fst_act).init_game_state f_strat s_strat turn) act
+    = g.transition (History_on_turn g.init_game_state fst_strat snd_strat (turn + 1)) act
+
+def Symm_Game_World.transition_blind_snd (g : Symm_Game_World α β) : Prop :=
+  ∀ f_strat s_strat: Strategy α β, ∀ fst_act : β, g.law [] fst_act →
+  let fst_strat : Strategy α β := (fun ini hist => if hist = [] then fst_act else s_strat (g.world_after_fst fst_act).init_game_state (hist.dropLast)) ;
+  let snd_strat : Strategy α β := (fun ini hist => f_strat (g.world_after_fst fst_act).init_game_state (hist.dropLast)) ;
+  ∀ turn : ℕ, ∀ act : β, g.transition (History_on_turn (g.world_after_fst fst_act).init_game_state f_strat s_strat turn) act
+    = g.transition (History_on_turn g.init_game_state fst_strat snd_strat (turn + 1)) act
+
+
+def Symm_Game_World.transition_blind (g : Symm_Game_World α β) : Prop :=
+ g.transition_blind_fst ∧ g.transition_blind_snd
+
+lemma Symm_Game_World.State_of_preconditioned
+  (g: Symm_Game_World α β)
+  (tb : g.transition_blind)
+  (fst_act: β)
+  (fst_act_legal: g.law [] fst_act)
+  (f_strat s_strat : Strategy α β)
+  (turn : ℕ):
+  let fst_strat : Strategy α β := (fun ini hist => if hist = [] then fst_act else s_strat (g.world_after_fst fst_act).init_game_state (hist.dropLast)) ;
+  let snd_strat : Strategy α β := (fun ini hist => f_strat (g.world_after_fst fst_act).init_game_state (hist.dropLast)) ;
+  g.state_on_turn fst_strat snd_strat (turn + 1) =
+  (g.world_after_fst fst_act).state_on_turn f_strat s_strat turn :=
+  by
+  intro fst_strat snd_strat
+  induction' turn with t ih
+  · dsimp [state_on_turn]
+    rw [if_pos (by decide)]
+    dsimp [history_on_turn, History_on_turn]
+    rw [if_pos (by rfl)]
+  · dsimp [state_on_turn]
+    by_cases q : Turn_fst (t + 1)
+    · rw [if_pos q]
+      rw [Turn_fst_not_step] at q
+      rw [if_neg q]
+      dsimp [history_on_turn]
+      have := g.History_of_preconditioned' fst_act f_strat s_strat t
+      dsimp at this
+      rw [this]
+      rw [List.dropLast_concat]
+      rw [← this]
+      clear this
+      have := tb.2 f_strat s_strat fst_act fst_act_legal
+      dsimp at this
+      specialize this t (f_strat (transition g [] fst_act) (History_on_turn (transition g [] fst_act) f_strat s_strat t))
+      rw [← this]
+      clear this
+      rfl
+    · rw [Turn_not_fst_iff_snd, Turn_snd_fst_step] at q
+      rw [if_pos q]
+      dsimp [history_on_turn]
+      rw [← Turn_fst_step, Turn_fst_not_step] at q
+      rw [if_neg q]
+      rw [if_neg (by apply History_on_turn_nonempty_of_succ)]
+      have := g.History_of_preconditioned' fst_act f_strat s_strat t
+      dsimp at this
+      rw [this]
+      rw [List.dropLast_concat]
+      rw [← this]
+      clear this
+      have := tb.1 f_strat s_strat fst_act fst_act_legal
+      dsimp at this
+      specialize this t (s_strat (transition g [] fst_act) (History_on_turn (transition g [] fst_act) f_strat s_strat t))
+      rw [← this]
+      clear this
+      rfl
+
+
+lemma Symm_Game_World.fst_legal_preconditioned'
+  (g: Symm_Game_World α β)
+  (fst_act: β)
+  (fst_act_legal: g.law [] fst_act)
+  (f_strat s_strat : Strategy α β)
+  (s_leg: Strategy_legal_snd (g.world_after_fst fst_act).init_game_state (fun x => (g.world_after_fst fst_act).law) f_strat s_strat)
+  (b : g.law_blind_fst')
+  :
+  let fst_strat : Strategy α β := (fun ini hist => if hist = [] then fst_act else s_strat (g.world_after_fst fst_act).init_game_state (hist.dropLast)) ;
+  let snd_strat : Strategy α β := (fun ini hist => f_strat (g.world_after_fst fst_act).init_game_state (hist.dropLast)) ;
+  Strategy_legal_fst g.init_game_state (fun x => g.law) fst_strat snd_strat :=
+  by
+  intro fst_strat snd_strat t tf
+  cases' t with t
+  · dsimp [History_on_turn]
+    rw [if_pos (by rfl)]
+    exact fst_act_legal
+  · rw [← b, Symm_Game_World.History_of_preconditioned']
+    · dsimp [History_on_turn]
+      rw [if_neg (by apply List.append_ne_nil_of_ne_nil_right ; exact List.cons_ne_nil fst_act [])]
+      rw [List.dropLast_concat]
+      apply s_leg
+      rw [Turn_snd_fst_step]
+      exact tf
+    · exact fst_act_legal
+
+
+lemma Symm_Game_World.snd_legal_preconditioned'
+  (g: Symm_Game_World α β)
+  (fst_act: β)
+  (fst_act_legal: g.law [] fst_act)
+  (f_strat s_strat : Strategy α β)
+  (f_leg: Strategy_legal_fst (g.world_after_fst fst_act).init_game_state (fun x => (g.world_after_fst fst_act).law) f_strat s_strat)
+  (b : g.law_blind_snd')
+  :
+  let fst_strat : Strategy α β := (fun ini hist => if hist = [] then fst_act else s_strat (g.world_after_fst fst_act).init_game_state (hist.dropLast)) ;
+  let snd_strat : Strategy α β := (fun ini hist => f_strat (g.world_after_fst fst_act).init_game_state (hist.dropLast)) ;
+  Strategy_legal_snd g.init_game_state (fun x => g.law) fst_strat snd_strat :=
+  by
+  intro fst_strat snd_strat t tf
+  cases' t with t
+  · contradiction
+  · rw [← b, Symm_Game_World.History_of_preconditioned']
+    · dsimp [History_on_turn]
+      rw [List.dropLast_concat]
+      apply f_leg
+      rw [Turn_fst_snd_step]
+      exact tf
+    · exact fst_act_legal
+
+
+inductive Symm_Game_World.Turn_isWL (g : Symm_Game_World α β) (f_strat s_strat : Strategy α β) (turn : ℕ) : Prop where
+| wf : Turn_fst turn → g.win_states (g.state_on_turn f_strat s_strat turn) → g.Turn_isWL f_strat s_strat turn
+| ws : Turn_snd turn → g.win_states (g.state_on_turn f_strat s_strat turn) → g.Turn_isWL f_strat s_strat turn
+
+
+def Symm_Game_World.isWL_wBound (g : Symm_Game_World α β) (T : ℕ) : Prop :=
+    ∀ f_strat s_strat : Strategy α β,
+    (f_leg : Strategy_legal_fst g.init_game_state (fun _ => g.law) f_strat s_strat) →
+    (s_leg : Strategy_legal_snd g.init_game_state (fun _ => g.law) f_strat s_strat) →
+    ∃ turn ≤ T, g.Turn_isWL f_strat s_strat turn
+
+def Symm_Game_World.nontrivial (g : Symm_Game_World α β) : Prop :=
+  ∀ f_strat s_strat : Strategy α β, ¬ (g.Turn_isWL f_strat s_strat 0)
+
+def Symm_Game_World.playable (g : Symm_Game_World α β) : Prop :=
+  ∃ f_strat s_strat : Strategy α β,
+  (Strategy_legal_fst g.init_game_state (fun _ => g.law) f_strat s_strat) ∧
+  (Strategy_legal_snd g.init_game_state (fun _ => g.law) f_strat s_strat)
+
+structure Symm_Game_World_Z (α β : Type u) extends Symm_Game_World α β where
+  lb : toSymm_Game_World.law_blind'
+  nt : toSymm_Game_World.nontrivial
+  tb : toSymm_Game_World.transition_blind
+  p : toSymm_Game_World.playable
+
+
+lemma Symm_Game_World_Z.conditioning_bound
+  (g : Symm_Game_World_Z α β)
+  {T : ℕ} (hg : g.isWL_wBound (T + 1))
+  (fst_act : β) (leg : g.law [] fst_act):
+  (g.world_after_fst fst_act).isWL_wBound T :=
+  by
+  intro f_strat s_strat f_leg s_leg
+  let fst_strat : Strategy α β := fun ini hist => if hist = [] then fst_act else s_strat (g.world_after_fst fst_act).init_game_state (hist.dropLast)
+  let snd_strat : Strategy α β := fun ini hist => f_strat (g.world_after_fst fst_act).init_game_state (hist.dropLast)
+  specialize hg fst_strat snd_strat _ _
+  · apply g.fst_legal_preconditioned' fst_act leg  f_strat s_strat s_leg g.lb.1
+  · apply g.snd_legal_preconditioned' fst_act leg  f_strat s_strat f_leg g.lb.2
+  · obtain ⟨t, t_bd, t_prop⟩ := hg
+    cases' t with t
+    · exfalso
+      exact (g.nt fst_strat snd_strat) t_prop
+    · rw [Nat.succ_le_succ_iff] at t_bd
+      use t
+      constructor
+      · exact t_bd
+      · cases' t_prop with tp c tp c c
+        · apply Symm_Game_World.Turn_isWL.ws
+          · rw [Turn_snd_fst_step] ; exact tp
+          · rw [← Symm_Game_World.State_of_preconditioned]
+            · rw [Symm_Game_World.world_after_fst_snd_win_states]
+              exact c
+            · exact g.tb
+            · exact leg
+        · apply Symm_Game_World.Turn_isWL.wf
+          · rw [Turn_fst_snd_step] ; exact tp
+          · rw [← Symm_Game_World.State_of_preconditioned]
+            · rw [Symm_Game_World.world_after_fst_win_states]
+              exact c
+            · exact g.tb
+            · exact leg
+
+lemma Symm_Game_World.conditioning_WLD_helper
+  (g : Symm_Game_World α β)
+  (hwld : g.has_WL)
+  (hnfw : ¬ g.is_fst_win):
+  g.is_snd_win :=
+  by
+  cases' hwld -- <;> { contradiction <|> assumption } --fails...
+  · contradiction
+  · assumption
+
+
+open Classical
+
+lemma Symm_Game_World_Z.conditioning_WLD
+  [Inhabited β]
+  (g : Symm_Game_World_Z α β)
+  (h : ∀ fst_act : β, g.law [] fst_act → (g.world_after_fst fst_act).has_WL) :
+  g.has_WL :=
+  by
+  by_cases qwf : ∃ f_act : β, g.law [] f_act ∧ (g.world_after_fst f_act).is_fst_win
+  · sorry
+  · push_neg at qwf
+    apply Symm_Game_World.has_WL.ws
+    let ws := fun (ini : α) hist  => if hh : hist = [] -- shouldn't happen, as snd strat
+                              then default -- dummy
+                              else let f_act := List.getLast hist hh
+                                   if H : g.law [] f_act -- should be the cases ?!?
+                                   then (Classical.choose ((g.world_after_fst f_act).conditioning_WLD_helper
+                                                            (h f_act H)
+                                                            (qwf f_act H)))
+                                          ini hist -- is it ?
+                                   else default
+    use ws
+    intro f_strat ws_leg f_leg
+    let f_act := f_strat g.init_game_state []
+    sorry
+
+
+lemma Symm_Game_World_Z.Zermelo
+  [Inhabited β]
+  (g : Symm_Game_World_Z α β)
+  {T : ℕ} (hg : g.isWL_wBound T)
+  : g.has_WL :=
+  by
+  revert g
+  induction' T with t ih
+  · intro g t0
+    dsimp [Symm_Game_World.isWL_wBound] at t0
+    obtain ⟨f_strat, s_strat, f_leg, s_leg⟩ := g.p
+    obtain ⟨t, tl0, t_end⟩ := t0 f_strat s_strat f_leg s_leg
+    rw [Nat.le_zero] at tl0
+    rw [tl0] at t_end
+    cases' t_end
+    · rename_i tt ttt; contradiction
+    · apply Symm_Game_World.has_WL.ws
+      use (fun _ _ => default)
+      intro f_strat' leg f_leg'
+      use 0
+      constructor
+      · decide
+      · constructor
+        · dsimp [Game.state_on_turn]
+          rename_i h ; exact h
+        · intro t ahhh ; contradiction
+  · intro g bd
+    apply Symm_Game_World_Z.conditioning_WLD
+    intro f_act f_leg
+    apply ih ((Symm_Game_World.world_after_fst g.toSymm_Game_World f_act))
+    · exact Game_World_wDraw.conditioning_bound g bd f_act f_leg hp.bl hp.nt hp.tb hp.wb
+    · exact pl
